Some progress in proving the final theorem.

core/TofinoPipeline.v
@@ -3,7 +3,6 @@ Require Import Poulet4.P4light.Semantics.Semantics.
 Require Import ProD3.core.Core.
 Require Import Poulet4.P4light.Architecture.Tofino.
 Require Import Poulet4.P4light.Architecture.Queue.
-Require Import Poulet4.P4light.Architecture.TrafficManager.
 Require Import Poulet4.P4light.Semantics.Typing.ValueTyping.
 Require Import ProD3.core.Tofino.
 
@@ -15,115 +14,86 @@ Notation P4Type := (@P4Type Info).
 Notation packet := (list bool).
 Notation fundef := (@fundef Info).
 
-Section Pipeline.
+Inductive programmable_block (ge : (@genv _ target)):
+  path -> ident -> fundef -> Prop :=
+| programmable_block_intro:
+  forall name fd pipe_class_name pipe_inst_path pipe_targs class_name inst_path targs,
+    PathMap.get ["main"; "pipe0"] (ge_inst ge) =
+      Some {|iclass:=pipe_class_name;
+             ipath:=pipe_inst_path; itargs:=pipe_targs|} ->
+    PathMap.get (pipe_inst_path ++ [name]) (ge_inst ge) =
+      Some {|iclass:=class_name; ipath:=inst_path; itargs:=targs|} ->
+    PathMap.get ([class_name; "apply"]) (ge_func ge) = Some fd ->
+    programmable_block ge inst_path name fd.
 
-  Variable ge : (@genv _ target).
+Definition programmable_block_sem :=
+  extern_state -> list Sval -> extern_state -> list Sval -> signal -> Prop.
 
-  Inductive programmable_block :
-    path -> ident -> fundef -> Prop :=
-  | programmable_block_intro:
-    forall name fd pipe_class_name pipe_inst_path pipe_targs class_name inst_path targs,
-      PathMap.get ["main"; "pipe0"] (ge_inst ge) =
-        Some {|iclass:=pipe_class_name;
-               ipath:=pipe_inst_path; itargs:=pipe_targs|} ->
-      PathMap.get (pipe_inst_path ++ [name]) (ge_inst ge) =
-        Some {|iclass:=class_name; ipath:=inst_path; itargs:=targs|} ->
-      PathMap.get ([class_name; "apply"]) (ge_func ge) = Some fd ->
-      programmable_block inst_path name fd.
-
-  Definition programmable_block_sem :=
-    extern_state -> list Sval -> extern_state -> list Sval -> signal -> Prop.
-
-  (*
-  Inductive ingress_pipeline:
-    extern_state -> packet_in -> extern_state -> packet_out -> Sval -> Prop :=
-  | ingress_pipeline_intro:
-    forall inprsr_path inprsr ingress_path ingress indeprsr_path indeprsr pin pout
-      m1 m2 m3 m4 m5 m6 s0 s1 s2 s3 s4
-      hdr1 hdr2 hdr3 ig_md1 ig_md2
-      payload ig_intr_md ig_intr_md_from_prsr1 ig_intr_md_for_dprsr1
-      ig_intr_md_for_dprsr2 ig_intr_md_for_tm1 ig_intr_md_for_tm2,
-      PathMap.set ["packet_out"] (ObjPout [])
-        (PathMap.set ["packet_in"] (ObjPin pin) s0) = s1 ->
-      programmable_block inprsr_path "ingress_parser" inprsr ->
-      exec_func ge read_ndetbit inprsr_path (m1, s1) inprsr nil [] (m2, s2)
-        [hdr1; ig_md1; ig_intr_md; ig_intr_md_for_tm1; ig_intr_md_from_prsr1]
-        SReturnNull ->
-      PathMap.get ["packet_in"] s2 = Some (ObjPin payload) ->
-      programmable_block ingress_path "ingress" ingress ->
-      exec_func ge read_ndetbit ingress_path (m3, s2) ingress []
-        [hdr1; ig_md1; ig_intr_md; ig_intr_md_from_prsr1; ig_intr_md_for_dprsr1;
-         ig_intr_md_for_tm1] (m4, s3)
-        [hdr2; ig_md2; ig_intr_md_for_dprsr2; ig_intr_md_for_tm2] SReturnNull ->
-      programmable_block indeprsr_path "ingress_deparser" indeprsr ->
-      exec_func ge read_ndetbit indeprsr_path (m5, s3) indeprsr nil
-        [hdr2; ig_md2; ig_intr_md_for_dprsr2; ig_intr_md] (m6, s4) [hdr3]
-        SReturnNull ->
-      PathMap.get ["packet_out"] s4 = Some (ObjPout pout) ->
-      ingress_pipeline s0 pin s4 (pout ++ payload) ig_intr_md_for_tm2.
-
-  Inductive egress_pipeline:
-    extern_state -> packet_in -> extern_state -> packet_out -> Prop :=
-  | egress_pipeline_intro:
-    forall eprsr_path eprsr egress_path egress edeprsr_path edeprsr pin pout
-      m1 m2 m3 m4 m5 m6 s0 s1 s2 s3 s4 hdr1 hdr2 hdr3 hdr4 eg_md1 eg_md2 eg_intr_md
-      eg_intr_md_from_prsr payload eg_intr_md_for_dprsr1 eg_intr_md_for_dprsr2
-      eg_intr_md_for_oport1 eg_intr_md_for_oport2,
-      PathMap.set ["packet_out"] (ObjPout [])
-        (PathMap.set ["packet_in"] (ObjPin pin) s0) = s1 ->
-      programmable_block eprsr_path "ingress_parser" eprsr ->
-      exec_func ge read_ndetbit eprsr_path (m1, s1) eprsr nil [] (m2, s2)
-        [hdr1; eg_md1; eg_intr_md; eg_intr_md_from_prsr] SReturnNull ->
-      PathMap.get ["packet_in"] s2 = Some (ObjPin payload) ->
-      programmable_block egress_path "ingress" egress ->
-      exec_func ge read_ndetbit egress_path (m3, s2) egress nil
-        [hdr1; eg_md1; eg_intr_md; eg_intr_md_from_prsr; eg_intr_md_for_dprsr1;
-         eg_intr_md_for_oport1] (m4, s3)
-        [hdr2; eg_md2; eg_intr_md_for_dprsr2; eg_intr_md_for_oport2] SReturnNull ->
-      programmable_block edeprsr_path "ingress" edeprsr ->
-      exec_func ge read_ndetbit edeprsr_path (m5, s3) edeprsr nil
-        [hdr3; eg_md2; eg_intr_md_for_dprsr2; eg_intr_md; eg_intr_md_from_prsr]
-        (m6, s4) [hdr4] SReturnNull ->
-      PathMap.get ["packet_out"] s4 = Some (ObjPout pout) ->
-      egress_pipeline s0 pin s4 (pout ++ payload).
-*)
-
-End Pipeline.
+Record pipeline_state := mkPipeSt {
+    parser_state: extern_state;
+    control_state: extern_state;
+    deparser_state: extern_state;
+  }.
 
 Inductive ingress_pipeline (inprsr ingress indeprsr: programmable_block_sem)
   (parser_ingress_cond ingress_deprsr_cond: list Sval -> list Sval -> Prop)
   (ingress_tm_cond: list Sval -> Sval -> Prop):
-  extern_state -> packet_in -> extern_state -> packet_out -> Sval -> Prop :=
+  pipeline_state -> packet -> pipeline_state -> packet -> Sval -> Prop :=
 | ingress_pipeline_intro:
-  forall pin pout s0 s1 s2 s3 s4 hdr1 hdr2 hdr3 ig_md1 ig_md2 payload
+  forall pin pout s1 s2 s3 s4 s5 s6 hdr1 hdr2 hdr3 ig_md1 ig_md2 payload
     rest1 rest2 rest3 rest4 for_tm,
-    PathMap.set ["packet_out"] (ObjPout [])
-      (PathMap.set ["packet_in"] (ObjPin pin) s0) = s1 ->
-    inprsr s1 [] s2 (hdr1 :: ig_md1 :: rest1) SReturnNull ->
+    inprsr (PathMap.set ["packet_in"] (ObjPin pin) s1) []
+      s2 (hdr1 :: ig_md1 :: rest1) SReturnNull ->
     PathMap.get ["packet_in"] s2 = Some (ObjPin payload) ->
     parser_ingress_cond rest1 rest2 ->
-    ingress s2 (hdr1 :: ig_md1 :: rest2) s3 (hdr2 :: ig_md2 :: rest3) SReturnNull ->
+    ingress s3 (hdr1 :: ig_md1 :: rest2) s4 (hdr2 :: ig_md2 :: rest3) SReturnNull ->
     ingress_deprsr_cond rest3 rest4 ->
-    indeprsr s3 (hdr2 :: ig_md2 :: rest4) s4 [hdr3] SReturnNull ->
-    PathMap.get ["packet_out"] s4 = Some (ObjPout pout) ->
+    indeprsr (PathMap.set ["packet_out"] (ObjPout []) s5)
+      (hdr2 :: ig_md2 :: rest4) s6 [hdr3] SReturnNull ->
+    PathMap.get ["packet_out"] s6 = Some (ObjPout pout) ->
     ingress_tm_cond rest3 for_tm ->
     ingress_pipeline inprsr ingress indeprsr parser_ingress_cond
-      ingress_deprsr_cond ingress_tm_cond s0 pin s4 (pout ++ payload) for_tm.
+      ingress_deprsr_cond ingress_tm_cond (mkPipeSt s1 s3 s5) pin
+      (mkPipeSt s2 s4 s6) (pout ++ payload) for_tm.
 
 Inductive egress_pipeline (eprsr egress edeprsr: programmable_block_sem)
   (parser_egress_cond egress_deprsr_cond: list Sval -> list Sval -> Prop) :
-  extern_state -> packet_in -> extern_state -> packet_out -> Prop :=
+  pipeline_state -> packet -> pipeline_state -> packet -> Prop :=
 | egress_pipeline_intro:
-  forall pin pout s0 s1 s2 s3 s4 hdr1 hdr2 hdr3 eg_md1 eg_md2 payload
+  forall pin pout s1 s2 s3 s4 s5 s6 hdr1 hdr2 hdr3 eg_md1 eg_md2 payload
     rest1 rest2 rest3 rest4,
-    PathMap.set ["packet_out"] (ObjPout [])
-      (PathMap.set ["packet_in"] (ObjPin pin) s0) = s1 ->
-    eprsr s1 [] s2 (hdr1 :: eg_md1 :: rest1) SReturnNull ->
+    eprsr (PathMap.set ["packet_in"] (ObjPin pin) s1) [] s2
+      (hdr1 :: eg_md1 :: rest1) SReturnNull ->
     PathMap.get ["packet_in"] s2 = Some (ObjPin payload) ->
     parser_egress_cond rest1 rest2 ->
-    egress s2 (hdr1 :: eg_md1 :: rest2) s3 (hdr2 :: eg_md2 :: rest3) SReturnNull ->
+    egress s3 (hdr1 :: eg_md1 :: rest2) s4 (hdr2 :: eg_md2 :: rest3) SReturnNull ->
     egress_deprsr_cond rest3 rest4 ->
-    edeprsr s3 (hdr2 :: eg_md2 :: rest4) s4 [hdr3] SReturnNull ->
-    PathMap.get ["packet_out"] s4 = Some (ObjPout pout) ->
+    edeprsr (PathMap.set ["packet_out"] (ObjPout []) s5)
+      (hdr2 :: eg_md2 :: rest4) s6 [hdr3] SReturnNull ->
+    PathMap.get ["packet_out"] s6 = Some (ObjPout pout) ->
     egress_pipeline eprsr egress edeprsr parser_egress_cond egress_deprsr_cond
-      s0 pin s4 (pout ++ payload).
+      (mkPipeSt s1 s3 s5) pin (mkPipeSt s2 s4 s6) (pout ++ payload).
+
+Section SWITCH.
+
+  Variable ingress_pipe: pipeline_state -> packet -> pipeline_state -> packet -> Sval -> Prop.
+  Variable egress_pipe: pipeline_state -> packet -> pipeline_state -> packet -> Prop.
+  Variable traffic_manager: Sval -> packet -> queue packet.
+
+  Inductive process_ingress_packets :
+    pipeline_state -> queue packet -> pipeline_state -> queue packet -> Prop :=
+  | pip_nil: forall st, process_ingress_packets st empty_queue st empty_queue
+  | pip_enque: forall st1 ps ps' md st2 p p' st3,
+      process_ingress_packets st1 ps st2 ps' ->
+      ingress_pipe st2 p st3 p' md ->
+      process_ingress_packets st1 (enque p ps) st3 (concat_queue ps' (traffic_manager md p')).
+
+  Inductive process_egress_packets :
+    pipeline_state -> queue packet -> pipeline_state -> queue packet -> Prop :=
+  | pep_nil: forall st, process_egress_packets st empty_queue st empty_queue
+  | pep_enque: forall st1 ps ps' st2 p p' st3,
+      process_egress_packets st1 ps st2 ps' ->
+      egress_pipe st2 p st3 p' ->
+      process_egress_packets st1 (enque p ps) st3 (enque p' ps').
+
+End SWITCH.
